language_formalisation/type_system/type_aux_lemmas.v
@@ -7,7 +7,8 @@ Add LoadPath "C:\Users\Ziga\Documents\Ziga_podatki\PHD\language_formalisation\op
 (* Add LoadPath "E:\Ziga_Podatki\faks\PHD\language_formalisation\substitution". *)
 (* Add LoadPath "E:\Ziga_Podatki\faks\PHD\language_formalisation\operational_semantics". *)
 
-Require Export syntax syntax_lemmas bidirectional substitution Omega Logic.
+Require Export syntax syntax_lemmas declarational substitution Omega Logic.
+Require Export subs_lemmas.
 
 Ltac inv H := inversion H; clear H; subst.
 
@@ -19,139 +20,84 @@ assert (i + 1 = S i) by omega.
 induction Γ; rewrite H; auto.
 Qed.
 
+
+
 (* Switch lemmas *)
-Fixpoint v_switch_checksafe
+Fixpoint v_switch_typesafe
   (Γ:ctx) i (Ai:vtype) j (Aj:vtype) (v:val) (A:vtype)
   (p_i : get_vtype_i Γ i = Some Ai) (p_j : get_vtype_i Γ j = Some Aj) 
   {struct v} :
-  vcheck Γ v A ->
-  vcheck (ctx_switch_vars Γ i j Ai Aj p_i p_j) (v_switch_vars v i j) A
+  has_vtype Γ v A ->
+  has_vtype (ctx_switch_vars Γ i j Ai Aj p_i p_j) (v_switch_vars v i j) A
 
-with v_switch_synthsafe
-  (Γ:ctx) i (Ai:vtype) j (Aj:vtype) (v:val) (A:vtype)
-  (p_i : get_vtype_i Γ i = Some Ai) (p_j : get_vtype_i Γ j = Some Aj)
-  {struct v}:
-  vsynth Γ v A ->
-  vsynth (ctx_switch_vars Γ i j Ai Aj p_i p_j) (v_switch_vars v i j) A
-
-with c_switch_checksafe 
+with c_switch_typesafe 
   (Γ:ctx) i (Ai:vtype) j (Aj:vtype) (c:comp) (C:ctype)
   (p_i : get_vtype_i Γ i = Some Ai) (p_j : get_vtype_i Γ j = Some Aj)
   {struct c}:
-  ccheck Γ c C -> 
-  ccheck (ctx_switch_vars Γ i j Ai Aj p_i p_j) (c_switch_vars c i j) C
+  has_ctype Γ c C -> 
+  has_ctype (ctx_switch_vars Γ i j Ai Aj p_i p_j) (c_switch_vars c i j) C
 
-with c_switch_synthsafe 
-  (Γ:ctx) i (Ai:vtype) j (Aj:vtype) (c:comp) (C:ctype)
-  (p_i : get_vtype_i Γ i = Some Ai) (p_j : get_vtype_i Γ j = Some Aj)
-  {struct c}:
-  csynth Γ c C -> 
-  csynth (ctx_switch_vars Γ i j Ai Aj p_i p_j) (c_switch_vars c i j) C
-
-with h_switch_checksafe
+with h_switch_typesafe
   (Γ:ctx) i (Ai:vtype) j (Aj:vtype) (h:hcases) (Σ:sig) (D:ctype)
   (p_i : get_vtype_i Γ i = Some Ai) (p_j : get_vtype_i Γ j = Some Aj)
   {struct h}:
-  hcheck Γ h Σ D ->
-  hcheck (ctx_switch_vars Γ i j Ai Aj p_i p_j) (h_switch_vars h i j) Σ D.
+  has_htype Γ h Σ D ->
+  has_htype (ctx_switch_vars Γ i j Ai Aj p_i p_j) (h_switch_vars h i j) Σ D.
 Proof.
 {
-clear v_switch_checksafe.
-clear c_switch_synthsafe.
-revert Γ i j Ai Aj A p_i p_j; induction v;
-intros Γ i j Ai Aj A p_i p_j orig.
-
-all: inv orig; try inv H.
+clear v_switch_typesafe.
+revert Γ i j Ai Aj A p_i p_j; induction v; intros Γ i j Ai Aj A p_i p_j orig.
+all: inv orig; try inv H; simpl.
 { (* relevant case *)
-  apply CheckVBySynth. simpl.
   destruct v as (name, num).
-  remember (num =? i) as cmpi.
-  induction cmpi; try apply SynthVar; simpl.
-  + simpl in H2. apply eq_sym in Heqcmpi. apply beq_nat_true in Heqcmpi.
-    rewrite Heqcmpi in H2. rewrite <-H2. apply eq_sym.
+  remember (num =? i) as cmpi. destruct cmpi; simpl.
+  + apply TypeVar. simpl.
+    simpl in *. apply eq_sym in Heqcmpi. apply beq_nat_true in Heqcmpi.
+    rewrite Heqcmpi in H1. rewrite <-H1. apply eq_sym.
     apply switch_ij_get_j.
-  + remember (num =? j) as cmpj.
-    induction cmpj.
-    * simpl in H2. apply eq_sym in Heqcmpj. apply beq_nat_true in Heqcmpj.
-      rewrite Heqcmpj in H2. apply SynthVar. rewrite <-H2. apply eq_sym.
+  + remember (num =? j) as cmpj. destruct cmpj.
+    * simpl in *. apply eq_sym in Heqcmpj. apply beq_nat_true in Heqcmpj.
+      rewrite Heqcmpj in H1. apply TypeVar. rewrite <-H1. apply eq_sym.
       apply switch_ij_get_i.
-    * rewrite (gets_same Γ (name,num) num) in H2. apply SynthVar.
-      rewrite <-H2. apply eq_sym. apply switch_ij_get_k.
-      apply eq_sym in Heqcmpi. apply beq_nat_false in Heqcmpi. auto.
-      apply eq_sym in Heqcmpj. apply beq_nat_false in Heqcmpj. auto.
-      simpl. apply eq_sym. apply beq_nat_refl.
+    * rewrite (gets_same Γ (name,num) num) in H1. apply TypeVar.
+      rewrite <-H1. apply eq_sym. apply switch_ij_get_k.
+      - apply eq_sym in Heqcmpi. apply beq_nat_false in Heqcmpi. auto.
+      - apply eq_sym in Heqcmpj. apply beq_nat_false in Heqcmpj. auto.
+      - simpl. apply eq_sym. apply beq_nat_refl.
 }
-+ apply CheckVBySynth. apply SynthUnit.
-+ apply CheckVBySynth. apply SynthInt.
-+ apply CheckInl. apply IHv. assumption.
-+ apply CheckInr. apply IHv. assumption.
-+ apply CheckVBySynth. apply SynthPair.
-  apply (v_switch_synthsafe _ i Ai j Aj _ _ p_i p_j) in H3. assumption.
-  apply (v_switch_synthsafe _ i Ai j Aj _ _ p_i p_j) in H5. assumption.
-+ apply CheckFun.
++ apply TypeUnit.
++ apply TypeInt.
++ apply TypeInl. auto.
++ apply TypeInr. auto.
++ apply TypePair; auto.
++ apply TypeFun. auto.
   apply (extend_get_proof _ A0) in p_i as pp_i.
   apply (extend_get_proof _ A0) in p_j as pp_j.
   rewrite (ctx_switch_extend1 Γ A0 i j Ai Aj p_i p_j pp_i pp_j).
-  apply c_switch_checksafe. assumption.
-+ apply CheckHandler.
-  * apply (extend_get_proof _ A0) in p_i as pp_i.
-    apply (extend_get_proof _ A0) in p_j as pp_j.
-    rewrite (ctx_switch_extend1 Γ A0 i j Ai Aj p_i p_j pp_i pp_j).
-    apply c_switch_checksafe. assumption.
-  * apply h_switch_checksafe. assumption.
-+ apply CheckVBySynth. apply SynthVAnnot. apply IHv. assumption.
-}
-{
-clear v_switch_synthsafe.
-clear c_switch_synthsafe.
-clear h_switch_checksafe.
-revert Γ i j Ai Aj A p_i p_j; induction v;
-intros Γ i j Ai Aj A p_i p_j orig; inv orig; try inv H; simpl.
-{ (* relevant case *)
-  destruct v as (name, num).
-  remember (num =? i) as cmpi.
-  induction cmpi; try apply SynthVar; simpl.
-  + simpl in H1. apply eq_sym in Heqcmpi. apply beq_nat_true in Heqcmpi.
-    rewrite Heqcmpi in H1. rewrite <-H1. apply eq_sym.
-    apply switch_ij_get_j.
-  + remember (num =? j) as cmpj.
-    induction cmpj.
-    * simpl in H1. apply eq_sym in Heqcmpj. apply beq_nat_true in Heqcmpj.
-      rewrite Heqcmpj in H1. apply SynthVar. rewrite <-H1. apply eq_sym.
-      apply switch_ij_get_i.
-    * rewrite (gets_same Γ (name,num) num) in H1. apply SynthVar.
-      rewrite <-H1. apply eq_sym. apply switch_ij_get_k.
-      apply eq_sym in Heqcmpi. apply beq_nat_false in Heqcmpi. auto.
-      apply eq_sym in Heqcmpj. apply beq_nat_false in Heqcmpj. auto.
-      simpl. apply eq_sym. apply beq_nat_refl.
-} 
-+ apply SynthUnit.
-+ apply SynthInt.
-+ apply SynthPair; apply IHv1 || apply IHv2; assumption.
-+ apply SynthVAnnot. apply v_switch_checksafe. assumption.
-}
-{
-clear c_switch_checksafe.
-clear h_switch_checksafe.
+  auto.
++ apply TypeHandler; auto.
+  apply (extend_get_proof _ A0) in p_i as pp_i.
+  apply (extend_get_proof _ A0) in p_j as pp_j.
+  rewrite (ctx_switch_extend1 Γ A0 i j Ai Aj p_i p_j pp_i pp_j).
+  auto.
++ apply TypeVAnnot. auto.
+}{
+clear c_switch_typesafe.
 revert Γ i j Ai Aj C p_i p_j; induction c;
 intros Γ i j Ai Aj C p_i p_j orig; inv orig; try inv H.
-+ remember (CTy A SigØ EqsØ) as C.
-  apply (CheckCBySynth _ _ C C); try reflexivity.
-  rewrite HeqC. apply SynthRet.
-  apply v_switch_synthsafe. assumption.
-+ apply (CheckCBySynth _ _ C' C'); try reflexivity.
-  apply (SynthΠMatch _ _ A B).
-  apply v_switch_synthsafe. assumption.
-  clear v_switch_checksafe.
-  apply (extend_get_proof _ A) in p_i as pp_i.
-  apply (extend_get_proof _ A) in p_j as pp_j.
-  apply (extend_get_proof _ B) in pp_i.
-  apply (extend_get_proof _ B) in pp_j.
-  assert (i+1+1=i+2) by omega. rewrite H in pp_i.
-  assert (j+1+1=j+2) by omega. rewrite H0 in pp_j.
-  rewrite (ctx_switch_extend2 _ _ _ _ _ _ _ p_i p_j pp_i pp_j).
-  apply c_switch_synthsafe; assumption.
-+ apply (CheckΣMatch _ _ A B); try apply v_switch_synthsafe; auto.
++ apply TypeRet. auto.
++ eapply TypeΠMatch.
+  - apply v_switch_typesafe. exact H4.
+  - apply (extend_get_proof _ A) in p_i as pp_i.
+    apply (extend_get_proof _ A) in p_j as pp_j.
+    apply (extend_get_proof _ B) in pp_i.
+    apply (extend_get_proof _ B) in pp_j.
+    assert (i+1+1=i+2) by omega. rewrite H in pp_i.
+    assert (j+1+1=j+2) by omega. rewrite H0 in pp_j.
+    rewrite (ctx_switch_extend2 _ _ _ _ _ _ _ p_i p_j pp_i pp_j).
+    apply IHc. assumption.
++ eapply TypeΣMatch. 
+  - apply v_switch_typesafe; exact H6.
   - apply (extend_get_proof _ A) in p_i as pp_i;
     apply (extend_get_proof _ A) in p_j as pp_j.
     rewrite (ctx_switch_extend1 Γ A i j Ai Aj p_i p_j pp_i pp_j).
@@ -160,56 +106,15 @@ intros Γ i j Ai Aj C p_i p_j orig; inv orig; try inv H.
     apply (extend_get_proof _ B) in p_j as pp_j.
     rewrite (ctx_switch_extend1 Γ B i j Ai Aj p_i p_j pp_i pp_j).
     apply IHc2. assumption.
-+ apply (CheckCBySynth _ _ C' C'); try reflexivity.
-  apply (SynthApp _ _ _ A C'). apply v_switch_synthsafe; assumption.
-  apply v_switch_checksafe. assumption.
-+ simpl. apply (CheckOp _ _ _ _ _ A_op B_op A Σ eqs); auto.
++ eapply TypeApp.
+  - apply v_switch_typesafe. exact H2.
+  - apply v_switch_typesafe. assumption.
++ eapply TypeOp. exact H5. auto.
   apply (extend_get_proof _ B_op) in p_i as pp_i.
   apply (extend_get_proof _ B_op) in p_j as pp_j.
   rewrite (ctx_switch_extend1 Γ B_op i j Ai Aj p_i p_j pp_i pp_j).
   apply IHc. assumption.
-+ apply (CheckCBySynth _ _ C' C'); try reflexivity.
-  apply SynthLetRec.
-  - apply (extend_get_proof _ A) in p_i as pp_i.
-    apply (extend_get_proof _ A) in p_j as pp_j.
-    apply (extend_get_proof _ (TyFun A C)) in pp_i.
-    apply (extend_get_proof _ (TyFun A C)) in pp_j.
-    assert (i+1+1=i+2) by omega. rewrite H in pp_i.
-    assert (j+1+1=j+2) by omega. rewrite H0 in pp_j.
-    rewrite (ctx_switch_extend2 _ _ _ _ _ _ _ p_i p_j pp_i pp_j).
-    apply IHc1. assumption.
-  - apply (extend_get_proof _ (TyFun A C)) in p_i as pp_i.
-    apply (extend_get_proof _ (TyFun A C)) in p_j as pp_j.
-    rewrite (ctx_switch_extend1 _ _ _ _ _ _  p_i p_j pp_i pp_j).
-    apply c_switch_synthsafe. assumption.
-+ apply (CheckCBySynth _ _ C' C'); try reflexivity.
-  apply (SynthHandle _ _ _ C).
-  - apply v_switch_synthsafe. assumption.
-  - apply IHc. assumption.
-+ apply (CheckCBySynth _ _ C' C'); try reflexivity.
-  apply SynthCAnnot. apply IHc. assumption.
-}
-{
-clear c_switch_synthsafe.
-clear h_switch_checksafe.
-revert Γ i j Ai Aj C p_i p_j; induction c;
-intros Γ i j Ai Aj C p_i p_j orig; inv orig; try inv H; simpl.
-+ apply SynthRet. apply v_switch_synthsafe. assumption.
-+ apply (SynthΠMatch _ _ A B).
-  apply v_switch_synthsafe. assumption.
-  clear v_switch_checksafe.
-  apply (extend_get_proof _ A) in p_i as pp_i.
-  apply (extend_get_proof _ A) in p_j as pp_j.
-  apply (extend_get_proof _ B) in pp_i.
-  apply (extend_get_proof _ B) in pp_j.
-  assert (i+1+1=i+2) by omega. rewrite H in pp_i.
-  assert (j+1+1=j+2) by omega. rewrite H0 in pp_j.
-  rewrite (ctx_switch_extend2 _ _ _ _ _ _ _ p_i p_j pp_i pp_j).
-  apply IHc. assumption.
-+ apply (SynthApp _ _ _ A C).
-  - apply v_switch_synthsafe. assumption.
-  - apply v_switch_checksafe. assumption.
-+ apply (SynthLetRec).
++ apply TypeLetRec.
   - apply (extend_get_proof _ A) in p_i as pp_i.
     apply (extend_get_proof _ A) in p_j as pp_j.
     apply (extend_get_proof _ (TyFun A C0)) in pp_i.
@@ -217,23 +122,21 @@ intros Γ i j Ai Aj C p_i p_j orig; inv orig; try inv H; simpl.
     assert (i+1+1=i+2) by omega. rewrite H in pp_i.
     assert (j+1+1=j+2) by omega. rewrite H0 in pp_j.
     rewrite (ctx_switch_extend2 _ _ _ _ _ _ _ p_i p_j pp_i pp_j).
-    apply c_switch_checksafe. assumption.
+    apply IHc1. assumption.
   - apply (extend_get_proof _ (TyFun A C0)) in p_i as pp_i.
     apply (extend_get_proof _ (TyFun A C0)) in p_j as pp_j.
     rewrite (ctx_switch_extend1 _ _ _ _ _ _  p_i p_j pp_i pp_j).
     apply IHc2. assumption.
-+ apply (SynthHandle _ _ _ C0 C).
-  - apply v_switch_synthsafe. assumption.
-  - apply c_switch_checksafe. assumption.
-+ apply SynthCAnnot. apply c_switch_checksafe. assumption.
-}
-{
-clear c_switch_synthsafe.
-clear h_switch_checksafe.
++ eapply TypeHandle.
+  - apply v_switch_typesafe. exact H2.
+  - apply IHc. assumption.
++ apply TypeCAnnot. apply IHc. assumption.
+}{
+clear h_switch_typesafe.
 revert Γ i j Ai Aj Σ D p_i p_j; induction h;
 intros Γ i j Ai Aj Σ D p_i p_j orig; inv orig; try inv H; simpl.
-apply CheckCasesØ.
-apply CheckCasesU.
+apply TypeCasesØ.
+apply TypeCasesU.
 + apply find_op_None_switch. assumption.
 + apply IHh. assumption.
 + apply (extend_get_proof _ (TyFun B_op D)) in p_i as pp_i.
@@ -243,40 +146,28 @@ apply CheckCasesU.
   assert (i+1+1=i+2) by omega. rewrite H in pp_i.
   assert (j+1+1=j+2) by omega. rewrite H0 in pp_j.
   rewrite (ctx_switch_extend2 _ _ _ _ _ _ _ p_i p_j pp_i pp_j).
-  apply c_switch_checksafe. assumption.
+  apply c_switch_typesafe. assumption.
 }
-Qed.
+Admitted.
 
 (* Switch lemmas *)
-Fixpoint v_switch10_checksafe
+Fixpoint v_switch10_typesafe
   (Γ:ctx) (A1:vtype) (A0:vtype) (v:val) (A:vtype)
   {struct v} :
-  vcheck (CtxU (CtxU Γ A1) A0) v A ->
-  vcheck (CtxU (CtxU Γ A0) A1) (v_switch_vars v 1 0) A
+  has_vtype (CtxU (CtxU Γ A1) A0) v A ->
+  has_vtype (CtxU (CtxU Γ A0) A1) (v_switch_vars v 1 0) A
 
-with v_switch10_synthsafe
-  (Γ:ctx) (A1:vtype) (A0:vtype) (v:val) (A:vtype)
-  {struct v}:
-  vsynth (CtxU (CtxU Γ A1) A0) v A ->
-  vsynth (CtxU (CtxU Γ A0) A1) (v_switch_vars v 1 0) A
-
-with c_switch10_checksafe 
+with c_switch10_typesafe 
   (Γ:ctx) (A1:vtype) (A0:vtype) (c:comp) (C:ctype)
   {struct c}:
-  ccheck (CtxU (CtxU Γ A1) A0) c C -> 
-  ccheck (CtxU (CtxU Γ A0) A1) (c_switch_vars c 1 0) C
+  has_ctype (CtxU (CtxU Γ A1) A0) c C -> 
+  has_ctype (CtxU (CtxU Γ A0) A1) (c_switch_vars c 1 0) C
 
-with c_switch10_synthsafe 
-  (Γ:ctx) (A1:vtype) (A0:vtype) (c:comp) (C:ctype)
-  {struct c}:
-  csynth (CtxU (CtxU Γ A1) A0) c C -> 
-  csynth (CtxU (CtxU Γ A0) A1) (c_switch_vars c 1 0) C
-
-with h_switch10_checksafe
+with h_switch10_typesafe
   (Γ:ctx) (A1:vtype) (A0:vtype) (h:hcases) (Σ:sig) (D:ctype)
   {struct h}:
-  hcheck (CtxU (CtxU Γ A1) A0) h Σ D ->
-  hcheck (CtxU (CtxU Γ A0) A1) (h_switch_vars h 1 0) Σ D.
+  has_htype (CtxU (CtxU Γ A1) A0) h Σ D ->
+  has_htype (CtxU (CtxU Γ A0) A1) (h_switch_vars h 1 0) Σ D.
 Proof.
 all: intro orig; remember (CtxU (CtxU Γ A1) A0) as Γ'.
 all: assert (get_vtype_i Γ' 1 = Some A1) as p_1.
@@ -286,11 +177,9 @@ all: try (rewrite HeqΓ'; simpl; f_equal).
 all: assert (ctx_switch_vars Γ' 1 0 A1 A0 p_1 p_0 = CtxU (CtxU Γ A0) A1).
 all: try (unfold ctx_switch_vars; rewrite HeqΓ'; simpl; f_equal).
 all: rewrite <-H.
-+ apply v_switch_checksafe. assumption.
-+ apply v_switch_synthsafe. assumption.
-+ apply c_switch_checksafe. assumption.
-+ apply c_switch_synthsafe. assumption.
-+ apply h_switch_checksafe. assumption.
++ apply v_switch_typesafe. assumption.
++ apply c_switch_typesafe. assumption.
++ apply h_switch_typesafe. assumption.
 Qed.
 
 Definition v_switch210_vars v := (v_switch_vars (v_switch_vars v 1 0) 2 1).
@@ -298,35 +187,23 @@ Definition c_switch210_vars c := (c_switch_vars (c_switch_vars c 1 0) 2 1).
 Definition h_switch210_vars h := (h_switch_vars (h_switch_vars h 1 0) 2 1).
 
 (* Switch lemmas *)
-Fixpoint v_switch210_checksafe
+Fixpoint v_switch210_typesafe
   (Γ:ctx) (A2 : vtype) (A1:vtype) (A0:vtype) (v:val) (A:vtype)
   {struct v} :
-  vcheck (CtxU (CtxU (CtxU Γ A2) A1) A0) v A ->
-  vcheck (CtxU (CtxU (CtxU Γ A0) A2) A1) (v_switch210_vars v) A
+  has_vtype (CtxU (CtxU (CtxU Γ A2) A1) A0) v A ->
+  has_vtype (CtxU (CtxU (CtxU Γ A0) A2) A1) (v_switch210_vars v) A
 
-with v_switch210_synthsafe
-  (Γ:ctx) (A2 : vtype) (A1:vtype) (A0:vtype) (v:val) (A:vtype)
-  {struct v}:
-  vsynth (CtxU (CtxU (CtxU Γ A2) A1) A0) v A ->
-  vsynth (CtxU (CtxU (CtxU Γ A0) A2) A1) (v_switch210_vars v) A
-
-with c_switch210_checksafe 
+with c_switch210_typesafe 
   (Γ:ctx) (A2 : vtype) (A1:vtype) (A0:vtype) (c:comp) (C:ctype)
   {struct c}:
-  ccheck (CtxU (CtxU (CtxU Γ A2) A1) A0) c C -> 
-  ccheck (CtxU (CtxU (CtxU Γ A0) A2) A1) (c_switch210_vars c) C
+  has_ctype (CtxU (CtxU (CtxU Γ A2) A1) A0) c C -> 
+  has_ctype (CtxU (CtxU (CtxU Γ A0) A2) A1) (c_switch210_vars c) C
 
-with c_switch210_synthsafe 
-  (Γ:ctx) (A2 : vtype) (A1:vtype) (A0:vtype) (c:comp) (C:ctype)
-  {struct c}:
-  csynth (CtxU (CtxU (CtxU Γ A2) A1) A0) c C -> 
-  csynth (CtxU (CtxU (CtxU Γ A0) A2) A1) (c_switch210_vars c) C
-
-with h_switch210_checksafe
+with h_switch210_typesafe
   (Γ:ctx) (A2 : vtype) (A1:vtype) (A0:vtype) (h:hcases) (Σ:sig) (D:ctype)
   {struct h}:
-  hcheck (CtxU (CtxU (CtxU Γ A2) A1) A0) h Σ D ->
-  hcheck (CtxU (CtxU (CtxU Γ A0) A2) A1) (h_switch210_vars h) Σ D.
+  has_htype (CtxU (CtxU (CtxU Γ A2) A1) A0) h Σ D ->
+  has_htype (CtxU (CtxU (CtxU Γ A0) A2) A1) (h_switch210_vars h) Σ D.
 Proof.
 all: intro orig; remember (CtxU (CtxU (CtxU Γ A2) A1) A0) as Γ'.
 all: remember (CtxU (CtxU (CtxU Γ A2) A0) A1) as Γ''.
@@ -344,14 +221,59 @@ all: try (unfold ctx_switch_vars; rewrite HeqΓ'; rewrite HeqΓ''; simpl; f_equa
 all: assert (ctx_switch_vars Γ'' 2 1 A2 A0 p'_2 p'_0 = Γ''').
 all: try (unfold ctx_switch_vars; rewrite HeqΓ''; rewrite HeqΓ'''; simpl; f_equal).
 all: rewrite <-H0.
-+ apply v_switch_checksafe. rewrite <-H.
-  apply v_switch_checksafe. assumption.
-+ apply v_switch_synthsafe. rewrite <-H.
-  apply v_switch_synthsafe. assumption.
-+ apply c_switch_checksafe. rewrite <-H.
-  apply c_switch_checksafe. assumption.
-+ apply c_switch_synthsafe. rewrite <-H.
-  apply c_switch_synthsafe. assumption.
-+ apply h_switch_checksafe. rewrite <-H.
-  apply h_switch_checksafe. assumption.
++ apply v_switch_typesafe. rewrite <-H.
+  apply v_switch_typesafe. assumption.
++ apply c_switch_typesafe. rewrite <-H.
+  apply c_switch_typesafe. assumption.
++ apply h_switch_typesafe. rewrite <-H.
+  apply h_switch_typesafe. assumption.
 Qed.
+
+
+
+Fixpoint v_shift_typesafe
+  (Γ:ctx) (A0:vtype) v A {struct v} :
+  has_vtype Γ v A ->
+  has_vtype (CtxU Γ A0) (Sub.v_shift v 1 0) A
+
+with c_shift_typesafe
+  (Γ:ctx) (A0:vtype) c C {struct c} :
+  has_ctype Γ c C ->
+  has_ctype (CtxU Γ A0) (Sub.c_shift c 1 0) C
+
+with h_shift_typesafe
+  (Γ:ctx) (A0:vtype) h Σ D {struct h} :
+  has_htype Γ h Σ D ->
+  has_htype (CtxU Γ A0) (Sub.h_shift h 1 0) Σ D.
+Proof.
+{
+clear v_shift_typesafe.
+revert Γ A0 A. induction v; intros Γ A0 A orig; simpl; inv orig.
++ destruct v as (name, num). simpl.
+  apply TypeVar. assert (num+1=S num) by omega. rewrite H.
+  simpl. assumption.
++ apply TypeUnit.
++ apply TypeInt.
++ apply TypeInl. apply IHv. assumption.
++ apply TypeInr. apply IHv. assumption.
++ apply TypePair. apply IHv1. assumption. apply IHv2. assumption.
++ apply TypeFun.
+  specialize (c_switch10_typesafe Γ A1 A0 (Sub.c_shift c 1 0) C) as Hs.
+  rewrite c_switch_1_0_shift_1_0 in Hs. auto.
++ apply TypeHandler.
+  - specialize (c_switch10_typesafe Γ A1 A0 (Sub.c_shift c 1 0) D) as Hs.
+    rewrite c_switch_1_0_shift_1_0 in Hs. auto.
+  - apply h_shift_typesafe. assumption.
++ apply TypeVAnnot. apply IHv. assumption.
+}{
+clear c_shift_typesafe.
+revert Γ A0 C. induction c; intros Γ A0 C orig; simpl; inv orig.
++ apply TypeRet. apply v_shift_typesafe. assumption.
++ eapply TypeΠMatch.
+  - apply v_shift_typesafe. exact H4.
+  - specialize (c_switch210_typesafe Γ A B A0 (Sub.c_shift c 1 0) C) as Hs.
+
+
+
+
+}
